

File: ws5.pr

**Lemma 1**  $[nat:ground] \forall x (\mathbf{S} \text{ nat}(x) \rightarrow gr(x)).$

**Proof.**

Induction<sub>0</sub>:  $\forall x (\mathbf{S} \text{ nat}(x) \rightarrow gr(x)).$

Hypothesis<sub>1</sub>: none.

Conclusion<sub>1</sub>:  $gr(0).$

Hypothesis<sub>1</sub>:  $gr(x)$  and  $\mathbf{S} \text{ nat}(x).$

Conclusion<sub>1</sub>:  $gr(\mathbf{s}(x)).$   $\square$

**Lemma 2**  $[add:ground:1] \forall x, y, z (\mathbf{S} \text{ add}(x, y, z) \rightarrow gr(x)).$

**Proof.**

Induction<sub>0</sub>:  $\forall x, y, z (\mathbf{S} \text{ add}(x, y, z) \rightarrow gr(x)).$

Hypothesis<sub>1</sub>: none.

Conclusion<sub>1</sub>:  $gr(0).$

Hypothesis<sub>1</sub>:  $gr(x)$  and  $\mathbf{S} \text{ add}(x, y, z).$

Conclusion<sub>1</sub>:  $gr(\mathbf{s}(x)).$   $\square$

**Lemma 3**  $[add:ground:2] \forall x, y, z (\mathbf{S} \text{ add}(x, y, z) \wedge gr(y) \rightarrow gr(z)).$

**Proof.**

Induction<sub>0</sub>:  $\forall x, y, z (\mathbf{S} \text{ add}(x, y, z) \rightarrow gr(y) \rightarrow gr(z)).$

Hypothesis<sub>1</sub>: none.

Conclusion<sub>1</sub>:  $gr(y) \rightarrow gr(y).$

Hypothesis<sub>1</sub>:  $gr(y) \rightarrow gr(z)$  and  $\mathbf{S} \text{ add}(x, y, z).$

Assumption<sub>2</sub>:  $gr(y). gr(z). gr(\mathbf{s}(z)).$

Thus<sub>2</sub>:  $gr(y) \rightarrow gr(\mathbf{s}(z)).$

Conclusion<sub>1</sub>:  $gr(y) \rightarrow gr(\mathbf{s}(z)).$   $\square$

**Lemma 4**  $[add:ground:3] \forall x, y, z (\mathbf{S} \text{ add}(x, y, z) \wedge gr(z) \rightarrow gr(y)).$

**Proof.**

Induction<sub>0</sub>:  $\forall x, y, z (\mathbf{S} \text{ add}(x, y, z) \rightarrow gr(z) \rightarrow gr(y)).$

Hypothesis<sub>1</sub>: none.

Conclusion<sub>1</sub>:  $gr(y) \rightarrow gr(y).$

Hypothesis<sub>1</sub>:  $gr(z) \rightarrow gr(y)$  and  $\mathbf{S} \text{ add}(x, y, z).$

Assumption<sub>2</sub>:  $gr(\mathbf{s}(z)). gr(z).$

Thus<sub>2</sub>:  $gr(\mathbf{s}(z)) \rightarrow gr(y).$

Conclusion<sub>1</sub>:  $gr(\mathbf{s}(z)) \rightarrow gr(y).$   $\square$

**Lemma 5**  $[add:types:2] \forall x, y, z (\mathbf{S} \text{ add}(x, y, z) \wedge \mathbf{S} \text{ nat}(y) \rightarrow \mathbf{S} \text{ nat}(z)).$

**Proof.**

Induction<sub>0</sub>:  $\forall x, y, z (\mathbf{S} \text{ add}(x, y, z) \rightarrow \mathbf{S} \text{ nat}(y) \rightarrow \mathbf{S} \text{ nat}(z)).$

Hypothesis<sub>1</sub>: none.

Conclusion<sub>1</sub>:  $\mathbf{S} \text{ nat}(y) \rightarrow \mathbf{S} \text{ nat}(y).$

Hypothesis<sub>1</sub>:  $\mathbf{S} \text{ nat}(y) \rightarrow \mathbf{S} \text{ nat}(z)$  and  $\mathbf{S} \text{ add}(x, y, z).$

Conclusion<sub>1</sub>:  $\mathbf{S} \text{ nat}(y) \rightarrow \mathbf{S} \text{ nat}(\mathbf{s}(z)).$   $\square$

**Lemma 6** [*add:types:3*]  $\forall x, y, z (\mathbf{S} \text{ add}(x, y, z) \wedge \mathbf{S} \text{ nat}(z) \rightarrow \mathbf{S} \text{ nat}(y))$ .

**Proof.**

Induction<sub>0</sub>:  $\forall x, y, z (\mathbf{S} \text{ add}(x, y, z) \rightarrow \mathbf{S} \text{ nat}(z) \rightarrow \mathbf{S} \text{ nat}(y))$ .

Hypothesis<sub>1</sub>: none.

Conclusion<sub>1</sub>:  $\mathbf{S} \text{ nat}(y) \rightarrow \mathbf{S} \text{ nat}(y)$ .

Hypothesis<sub>1</sub>:  $\mathbf{S} \text{ nat}(z) \rightarrow \mathbf{S} \text{ nat}(y)$  and  $\mathbf{S} \text{ add}(x, y, z)$ .

Assumption<sub>2</sub>:  $\mathbf{S} \text{ nat}(\mathbf{s}(z))$ .  $\mathbf{D} \mathbf{S} \text{ nat}(\mathbf{s}(z))$  by completion.

Thus<sub>2</sub>:  $\mathbf{S} \text{ nat}(\mathbf{s}(z)) \rightarrow \mathbf{S} \text{ nat}(y)$ .

Conclusion<sub>1</sub>:  $\mathbf{S} \text{ nat}(\mathbf{s}(z)) \rightarrow \mathbf{S} \text{ nat}(y)$ .  $\square$

**Lemma 7** [*nat:termination*]  $\forall x (\mathbf{S} \text{ nat}(x) \rightarrow \mathbf{T} \text{ nat}(x))$ .

**Proof.**

Induction<sub>0</sub>:  $\forall x (\mathbf{S} \text{ nat}(x) \rightarrow \mathbf{T} \text{ nat}(x))$ .

Hypothesis<sub>1</sub>: none.

Conclusion<sub>1</sub>:  $\mathbf{T} \text{ nat}(0)$ .

Hypothesis<sub>1</sub>:  $\mathbf{T} \text{ nat}(x)$  and  $\mathbf{S} \text{ nat}(x)$ .  $\mathbf{D} \mathbf{T} \text{ nat}(\mathbf{s}(x))$  by completion.

Conclusion<sub>1</sub>:  $\mathbf{T} \text{ nat}(\mathbf{s}(x))$ .  $\square$

**Lemma 8** [*add:termination:1*]  $\forall x, y, z (\mathbf{S} \text{ nat}(x) \rightarrow \mathbf{T} \text{ add}(x, y, z))$ .

**Proof.**

Induction<sub>0</sub>:  $\forall x (\mathbf{S} \text{ nat}(x) \rightarrow \forall y, z \mathbf{T} \text{ add}(x, y, z))$ .

Hypothesis<sub>1</sub>: none.

Conclusion<sub>1</sub>:  $\forall y, z \mathbf{T} \text{ add}(0, y, z)$ .

Hypothesis<sub>1</sub>:  $\forall y, z \mathbf{T} \text{ add}(x, y, z)$  and  $\mathbf{S} \text{ nat}(x)$ .

Conclusion<sub>1</sub>:  $\forall y, z \mathbf{T} \text{ add}(\mathbf{s}(x), y, z)$ .  $\square$

**Lemma 9** [*add:termination:2*]  $\forall x, y, z (\mathbf{S} \text{ nat}(z) \rightarrow \mathbf{T} \text{ add}(x, y, z))$ .

**Proof.**

Induction<sub>0</sub>:  $\forall z (\mathbf{S} \text{ nat}(z) \rightarrow \forall x, y \mathbf{T} \text{ add}(x, y, z))$ .

Hypothesis<sub>1</sub>: none.

Conclusion<sub>1</sub>:  $\forall x, y \mathbf{T} \text{ add}(x, y, 0)$ .

Hypothesis<sub>1</sub>:  $\forall v_0, y \mathbf{T} \text{ add}(v_0, y, x)$  and  $\mathbf{S} \text{ nat}(x)$ .

Conclusion<sub>1</sub>:  $\forall v_0, y \mathbf{T} \text{ add}(v_0, y, \mathbf{s}(x))$ .  $\square$

**Lemma 10** [*add:termination:3*]  $\forall x, y, z (\mathbf{S} \text{ add}(x, y, z) \rightarrow \mathbf{T} \text{ add}(x, y, z))$ .

**Proof.**

Induction<sub>0</sub>:  $\forall x, y, z (\mathbf{S} \text{ add}(x, y, z) \rightarrow \mathbf{T} \text{ add}(x, y, z))$ .

Hypothesis<sub>1</sub>: none.

Conclusion<sub>1</sub>:  $\mathbf{T} \text{ add}(0, y, y)$ .

Hypothesis<sub>1</sub>:  $\mathbf{T} \text{ add}(x, y, z)$  and  $\mathbf{S} \text{ add}(x, y, z)$ .

Conclusion<sub>1</sub>:  $\mathbf{T} \text{ add}(\mathbf{s}(x), y, \mathbf{s}(z))$ .  $\square$